Prove that compactness implies WKL

theories/WKL.v
@@ -1,4 +1,34 @@
-Require Import Undecidability.FOLC.GenCompleteness.
+Require Import Undecidability.FOLC.GenCompleteness Lia Nat.
+
+Definition max_list_with {A} (f : A -> nat) : list A -> nat :=
+  fix go l :=
+  match l with
+  | [] => 0
+  | x :: l => Nat.max (f x) (go l)
+  end.
+Notation max_list := (max_list_with (fun x => x)).
+
+Lemma max_list_spec l :
+  l <> nil -> In (max_list l) l. 
+Proof.
+  destruct l as [ | x l] using rev_ind; try congruence.
+  clear IHl. intros _. induction l; cbn in *.
+  - left. lia.
+  - destruct (Nat.max_dec a (max_list (l ++ [x]))) as [H1 | H1].
+    + now left.
+    + right. rewrite H1 in *. eauto.
+Qed.
+
+Lemma max_list_spec' x l :
+  In x l -> x <= max_list l.
+Proof.
+  intros H.
+  induction l in x, H |- *.
+  - inv H.
+  - inv H; cbn.
+    + lia. 
+    + eapply IHl in H0. lia.
+Qed.
 
 (** ** WKL  *)
 
@@ -58,72 +88,454 @@ Definition model_existence (Cond : forall Sigma D, @interp Sigma D -> Prop) :=
   forall {HdF : eq_dec Funcs} {HdP : eq_dec Preds},
   forall {HeF : enumT Funcs} {HeP : enumT Preds},
   forall T (T_closed : closed_T T), consistent T ->
-  exists (D : Type) (I : @interp Sigma D), inhabited (eq_dec D) /\ inhabited (enumT D) /\
-                                      Cond Sigma D I /\ 
-                                      forall phi, closed phi -> phi ∈ T -> forall rho, rho ⊨ phi.
+                               has_model (Cond Sigma) T.
 
-Goal model_existence (@SM).
-Proof.
-  intros Sigma HdF HdP HeF HeP T T_closed T_cons.
-  pose proof (@model_bot_correct Sigma HdF HdP HeF HeP T T_closed).
-  exists (@term Sigma). eexists.
-  setoid_rewrite <- H.
-  repeat split; try exact _.
-  - eapply model_bot_classical.
-  - now eapply model_bot_standard.
-  - intros. eapply Out_T_sub. cbn. 
-    setoid_rewrite subst_unused_closed. 2:eauto.
-    asimpl. eassumption.
-Qed.
-
-Definition model_existence' (Cond : forall Sigma D, @interp Sigma D -> Prop) :=
-  forall {Sigma : Signature},
-  forall {HdF : eq_dec Funcs} {HdP : eq_dec Preds},
-  forall {HeF : enumT Funcs} {HeP : enumT Preds},
-  forall T (T_closed : closed_T T), consistent T ->
-  exists (D : Type) (I : @interp Sigma D) rho, inhabited (eq_dec D) /\ inhabited (enumT D) /\
-                                    Cond Sigma D I /\ forall phi, phi ∈ T -> rho ⊨ phi.
-
-Lemma modex_standard :
-  model_existence' (@SM).
-Proof.
-  intros Sigma HdF HdP HeF HeP T T_closed T_cons.
-  pose proof (@model_bot_correct Sigma HdF HdP HeF HeP T T_closed).
-  exists (@term Sigma). eexists. exists ids.
-  setoid_rewrite <- H.
-  repeat split; try exact _.
-  - eapply model_bot_classical.
-  - now eapply model_bot_standard.
-  - intros. eapply Out_T_sub. cbn. asimpl. assumption.
-Qed.
+Definition countable (X : Type) := inhabited (eq_dec X) /\ inhabited (enumT X).
 
 Definition compactness (C : forall Sigma D, @interp Sigma D -> Prop) :=
   forall {Sigma : Signature},
   forall {HdF : eq_dec Funcs} {HdP : eq_dec Preds},
   forall {HeF : enumT Funcs} {HeP : enumT Preds},
   forall T (T_closed : closed_T T),
-  (forall Gamma, Gamma ⊏ T -> exists D (I : interp D) rho, SM I /\ forall phi, phi el Gamma -> rho ⊨ phi)
-  -> exists D (I : interp D) rho, C Sigma D I /\ forall phi, phi ∈ T -> rho ⊨ phi.
+  (forall Gamma, Gamma ⊏ T -> has_model SM (fun x => In x Gamma))
+  -> has_model (C Sigma) T.
+
+Lemma modex_standard :
+  model_existence (fun Sigma D I => @SM Sigma D I /\ countable D).
+Proof.
+  intros Sigma HdF HdP HeF HeP T T_closed T_cons.
+  pose proof (@model_bot_correct Sigma HdF HdP HeF HeP T T_closed).
+  exists (@term Sigma). eexists. exists ids.
+  setoid_rewrite <- H.
+  repeat split; try exact _.
+  - intros. eapply Out_T_sub. cbn. asimpl. assumption.
+  - eapply model_bot_classical.
+  - now eapply model_bot_standard.
+Qed.
 
 Lemma modex_compact (C : forall Sigma D, @interp Sigma D -> Prop) :
-  model_existence' C -> compactness C.
+  model_existence C -> compactness C.
 Proof.
   intros HM Sigma HdF HdP HeF HeP T T_closed H.
-  apply HM in T_closed as (D & I & rho & _ & _ & HI); trivial.
+  apply HM in T_closed as (D & I & rho & HI); trivial.
   + intros [Gamma [H1 H2]]. apply H in H1 as (D & I & rho & H3 & H4).
-    apply Soundness' in H2. apply H3. now apply (H2 D I H3 rho).
+    apply Soundness' in H2. apply H4. now apply (H2 D I H4 rho).
   + now exists D, I, rho.
 Qed.
 
 Lemma compact_standard :
-  compactness (@SM).
+  compactness (fun Sigma D I => @SM Sigma D I /\ countable D).
 Proof.
   apply modex_compact. apply modex_standard.
 Qed.
 
-Definition DM `{Signature} D (I : interp D) := classical I /\ standard_bot I /\ GenTarski.decidable I.
+Definition decidable_model := 
+fun (Sigma : Signature) (D : Type) (I : interp D) => exists f : forall P, vector D (pred_ar P) -> bool, forall P, forall v : vector D (pred_ar P), f P v = true <-> i_P v.
 
-(* Goal model_existence_dec -> WKL. *)
-(* Proof. *)
-(*   intros me T Ht. *)
-(*   specialize (me (B_S False ltac:(tauto) nat (fun _ => 0)) _ _ _ _). *)
+Definition DM `{Signature} D (I : interp D) := SM I /\ countable D /\ decidable_model I.
+
+Definition count_sig := @B_S False ltac:(tauto) nat (fun n => 0).
+
+Definition Neg `{Signature} phi := Impl phi Fal.
+
+Definition Or `{Signature} phi psi := Impl (Neg phi) psi.
+
+Definition And `{Signature} phi psi := Neg (Or (Neg phi) (Neg psi)).
+
+Lemma Neg_sat `{Signature} D (I : interp D) rho phi :
+  standard_bot I ->
+  rho ⊨ Neg phi <-> ~ rho ⊨ phi.
+Proof.
+  firstorder.
+Qed.
+
+Notation omniscient_on I phi := (forall (rho : env _), dec (rho ⊨ phi)).
+Definition omniscient := fun (Sigma : Signature) (D : Type) (I : interp D) => inhabited (forall phi, omniscient_on I phi).
+
+Lemma omniscient_on_Neg `{Signature} D (I : interp D) phi :
+  standard_bot I ->
+  omniscient_on I phi -> omniscient_on I (Neg phi).
+Proof.
+  intros ? ? ?. destruct (X rho); cbn; firstorder.
+Qed.
+Hint Resolve omniscient_on_Neg : core.
+
+Lemma Or_sat `{Signature} D (I : interp D) rho phi psi :
+  standard_bot I -> inhabited (omniscient_on I phi) -> inhabited (omniscient_on I psi) ->
+  rho ⊨ Or phi psi <-> rho ⊨ phi \/ rho ⊨ psi.
+Proof.
+  firstorder.
+Qed.
+
+Lemma omniscient_on_Or `{Signature} D (I : interp D) phi psi :
+  standard_bot I ->
+  omniscient_on I phi ->
+  omniscient_on I psi ->
+  omniscient_on I (Or phi psi).
+Proof.
+  firstorder.
+Qed.
+Hint Resolve omniscient_on_Or : core.
+
+Lemma And_sat `{Signature} D (I : interp D) rho phi psi :
+  standard_bot I -> inhabited (omniscient_on I phi) -> inhabited (omniscient_on I psi) ->
+  rho ⊨ And phi psi <-> rho ⊨ phi /\ rho ⊨ psi.
+Proof.
+  intros ? [] [].
+  split; unfold And; rewrite Neg_sat, Or_sat; eauto; firstorder.
+Qed.
+
+Lemma omniscient_on_And `{Signature} D (I : interp D) phi psi :
+  standard_bot I ->
+  omniscient_on I phi ->
+  omniscient_on I psi ->
+  omniscient_on I (And phi psi).
+Proof.
+  intros. destruct (X rho), (X0 rho); cbn; firstorder.
+Qed.
+Hint Resolve omniscient_on_And : core.
+
+Fixpoint fExists `{Signature} (l : list form) :=
+  match l with
+  | [] => Fal
+  | phi :: l => Or phi (fExists l)
+  end.
+
+Lemma to_False_iff {P : Prop} :
+  (P -> False) -> (P <-> False).
+Proof.
+  tauto.
+Qed.
+
+Lemma omniscient_on_fExists_sat `{Signature} D (I : interp D) l :
+  standard_bot I -> (forall phi, In phi l -> omniscient_on I phi) ->
+  omniscient_on I (fExists l).
+Proof.
+  intros SB omn rho.
+  induction l  as [ | phi] in SB, omn, rho |- *.
+  - firstorder.
+  - cbn - [Or].
+    edestruct (omn phi); eauto.
+    + left. rewrite Or_sat; eauto. 
+    + edestruct IHl; eauto.
+      * left. rewrite Or_sat; eauto.
+      * right. rewrite Or_sat; eauto. firstorder.
+Qed.
+
+Lemma fExists_sat' `{Signature} D (I : interp D) rho l :
+  standard_bot I -> (forall phi, In phi l -> omniscient_on I phi) ->
+  rho ⊨ fExists l <-> exists phi, In phi l /\ rho ⊨ phi.
+Proof.
+  intros SB omn.
+  induction l.
+  - firstorder.
+  - cbn - [Or].
+    rewrite Or_sat, IHl; eauto.
+    split.
+    + intros [ | [? []]]; eauto.
+    + intros [? [[-> | ]]]; eauto.
+    + econstructor. eapply omniscient_on_fExists_sat; eauto.
+Qed.
+
+Lemma fExists_sat `{Signature} D (I : interp D) rho l :
+  standard_bot I -> omniscient I ->
+  rho ⊨ fExists l <-> exists phi, In phi l /\ rho ⊨ phi.
+Proof.
+  intros ? []. eapply fExists_sat'; eauto.
+Qed.
+
+Fixpoint fAll `{Signature} (l : list form) :=
+  match l with
+  | [] => Impl Fal Fal
+  | phi :: l => And phi (fAll l)
+  end.
+
+Lemma omniscient_on_fAll_sat `{Signature} D (I : interp D) l :
+  standard_bot I -> (forall phi, In phi l -> omniscient_on I phi) ->
+  omniscient_on I (fAll l).
+Proof.
+  intros SB omn rho.
+  induction l  as [ | phi] in SB, omn, rho |- *.
+  - firstorder.
+  - cbn - [And].
+    edestruct (omn phi); eauto.
+    + edestruct IHl; eauto.
+      * left. rewrite And_sat; eauto.
+      * right. rewrite And_sat; eauto. firstorder.
+    + right. rewrite And_sat; eauto. firstorder.
+Qed.
+
+Lemma fAll_sat' `{Signature} D (I : interp D) rho l :
+  standard_bot I -> (forall phi, In phi l -> (omniscient_on I phi)) ->
+  rho ⊨ fAll l <-> forall phi, In phi l -> rho ⊨ phi.
+Proof.
+  intros SB omn.
+  induction l.
+  - firstorder.
+  - cbn - [And].
+    rewrite And_sat, IHl; eauto.
+    split.
+    + intros [] ? [-> | ]; eauto.
+    + eauto 9.
+    + econstructor. eapply omniscient_on_fAll_sat; eauto.
+Qed.
+
+Lemma fAll_sat `{Signature} D (I : interp D) rho l :
+  standard_bot I -> omniscient I ->
+  rho ⊨ fAll l <-> forall phi, In phi l -> rho ⊨ phi.
+Proof.
+  intros ? []. eapply fAll_sat'; eauto.
+Qed.
+
+Definition listable {X} (p : X -> Prop) := { L : list X | forall x, p x <-> In x L}.
+
+Lemma listable_list_length :
+  forall k : nat, listable (fun x : list bool => length x = k).
+Proof.
+  induction k as [ | k [L IH] ].
+  - exists [ [] ]. intros [] ; cbv ; firstorder. inv H.
+  - exists (map (cons true) L ++ map (cons false) L).
+    intros l.
+    rewrite in_app_iff, !in_map_iff.
+    repeat setoid_rewrite <- IH.
+    destruct l as [ | [] ].
+    + cbn. split. inversion 1. firstorder congruence.
+    + cbn. split. 
+      * inversion 1. eauto.
+      * firstorder; now inv H.
+    + cbn. split. 
+      * inversion 1. eauto.
+      * firstorder; now inv H.
+Qed.
+
+Notation nat := (nat).
+
+Fixpoint mapi {X Y} (f : nat -> X -> Y) (l : list X) i :=
+  match l with
+  | [] => []
+  | x :: l => f i x :: mapi f l (S i)
+  end.
+
+Lemma in_mapi_iff {X Y} (f : nat -> X -> Y) l y i :
+  In y (mapi f l i) <-> exists x j, f (j + i) x = y /\ nth_error l j = Some x.
+Proof.
+  induction l as [ | x l] in i |- *; cbn.
+  - firstorder. destruct x0; inv H0.
+  - rewrite IHl. intuition subst.
+    + now exists x, 0. 
+    + destruct H0 as (x' & j & H1 & H2).
+      exists x', (S j). split. rewrite <- H1; f_equal. lia. now cbn.
+    + destruct H as (x' & [ | j] & H1 & H2); cbn in *.
+      * inv H2. eauto.
+      * right. exists x', j. split. rewrite <- H1; f_equal. lia. now cbn.
+Qed.
+
+Lemma mapi_app {X Y} (f : nat -> X -> Y) (l1 l2 : list X) i :
+  mapi f (l1 ++ l2) i = mapi f l1 i ++ mapi f l2 (length l1 + i).
+Proof.
+  induction l1 in l2, i |- *; cbn.
+  - reflexivity.
+  - rewrite IHl1. repeat f_equal. lia.
+Qed.
+
+Lemma infinite_iff (T : tree) :
+  infinite_tree T <-> forall k : nat, exists a : list bool, T a /\ | a | = k.
+Proof.
+  split.
+  - intros H k. destruct (H k) as (? & ? & ?).
+    exists (firstn k x). split. eapply tree_p. eapply T. 2:eauto.
+    rewrite <- (firstn_skipn k x) at 2. eexists; eauto.
+    rewrite firstn_length. lia.
+  - intros H k. destruct (H k) as (? & ? & ?). exists x. split. eauto. lia.
+Qed.
+
+Section WKL.
+
+  Variable T : tree.
+  Variable T_D : list bool -> bool.
+  Variable HD : forall x, T_D x = true <-> T x.
+
+  Definition phi n := fExists (map (fun l => fAll (mapi (fun i (b : bool) => if b then @Pred count_sig i Vector.nil else Neg (@Pred count_sig i Vector.nil)) l 0)) (filter T_D (proj1_sig (listable_list_length n)))).
+
+  Definition Th psi := exists n, psi = phi n.
+
+  Lemma phi_down_S D (I : interp D) rho n :
+    @standard_bot count_sig D I -> omniscient I ->
+      rho ⊨ phi (S n) -> rho ⊨ phi n.
+  Proof.
+    intros SB omn H.
+    eapply fExists_sat in H as (phi' & H1 & H); eauto.
+    eapply in_map_iff in H1 as (l & <- & [H3 H4] % in_filter_iff); eauto.
+    rewrite fAll_sat in H; eauto.
+    destruct (listable_list_length (S n)) as [L HL].
+    cbn in *. eapply HL in H3.
+    destruct l as [ | b l _] using rev_ind; try now inv H3.
+    rewrite app_length in H3. cbn in H3. rewrite plus_comm in H3. inv H3.
+    eapply fExists_sat; eauto.
+    eexists. split.
+    - eapply in_map_iff. exists l. split. reflexivity.
+      eapply in_filter_iff. split.
+      destruct listable_list_length as [L' HL'].
+      + cbn. eapply HL'. reflexivity.
+      + eapply HD in H4. eapply HD.
+        eapply tree_p. eapply T. 2:exact H4. exists [b]; eauto.
+    - eapply fAll_sat; eauto. intros. eapply H. rewrite mapi_app. eapply in_app_iff. eauto.
+  Qed.
+
+  Lemma phi_down D (I : interp D) rho n m :
+    @standard_bot count_sig D I -> omniscient I ->
+    rho ⊨ phi n -> n >= m -> rho ⊨ phi m.
+  Proof.
+    intros SB omn H1 H2. induction H2.
+    - eauto.
+    - eapply IHle, phi_down_S, H1; eauto.
+  Qed.
+
+  (* Induktionsbeispiele von Kathrin *)
+
+  Lemma decidable_to_omniscient {Σ : Signature} (I : interp unit) :
+    decidable_model I -> standard_bot I -> omniscient I.
+  Proof.
+    intros [d Hd] SB. econstructor. intros phi rho.
+    induction phi in rho |- *; cbn.
+    - firstorder.
+    - destruct (d P (Vector.map (eval rho) t)) eqn:E.
+      + left. now eapply Hd.
+      + right. intros ? % Hd. congruence.
+    - destruct (IHphi1 rho), (IHphi2 rho); firstorder.
+    - destruct (IHphi (tt .: rho)). left; now intros [].
+      right. firstorder.
+  Qed.
+
+  Lemma omniscient_to_classical {Σ : Signature} D (I : interp D) :
+    omniscient I -> classical I.
+  Proof.
+    intros [d] rho phi psi. cbn.
+    destruct (d phi rho), (d psi rho); tauto.
+  Qed.
+
+  Lemma compact_DM_WKL :
+    compactness (@DM) -> infinite_tree T -> infinite_path T.
+  Proof.
+    intros compact infT.
+    destruct (compact count_sig _ _ _ _ Th) as (D & I & rho & H & (classI & standI) & (eq_dec_D & enum_D) & (f & decI)).
+    - intros psi n [m ->]. unfold phi.
+      induction proj1_sig; cbn.
+      + econstructor.
+      + destruct (T_D a); repeat econstructor; eauto.
+        generalize 0 as k.
+        induction a; intros; cbn; try destruct a; repeat econstructor.
+        * intros. inv X.
+        * eauto.
+        * intros. inv X.
+        * eauto.
+    - intros Γ HΓ.
+      assert (exists L, Γ = map phi L) as [L ->]. {
+        induction Γ as [ | psi Γ].
+        - now exists [].
+        - destruct IHΓ as [L]. firstorder.
+          subst. specialize (HΓ psi (or_introl eq_refl)) as [n Hn].
+          exists (n :: L). subst. reflexivity.
+      }
+      pose (m := max_list L).
+      rewrite infinite_iff in infT.
+      destruct (infT m) as (l & Hl & Hs).
+      exists unit.
+      unshelve epose (I := _ : @interp count_sig unit).
+      + econstructor.
+        * intros [].
+        * cbn. intros n _.
+          exact (nth n l false = true).
+        * exact False.
+      + exists I.
+        assert (omn : omniscient I).
+        { eapply decidable_to_omniscient.
+          unshelve eexists.
+          -- cbn. intros n _.
+             exact (nth n l false).
+          -- cbn. reflexivity.
+          -- now cbv.
+        }
+        assert (SB : standard_bot I).
+        { now cbv. }
+        exists (fun _ => tt). repeat split; eauto.
+        * intros phi (n & <- & H) % in_map_iff.
+          assert (Hn : n <= m) by now eapply max_list_spec'.
+          eapply phi_down; eauto.  
+          eapply fExists_sat; eauto. eexists. split.
+          -- eapply in_map_iff. exists l. split. reflexivity.
+             eapply in_filter_iff. split.
+             destruct listable_list_length. cbn. now eapply i.
+             now eapply HD.
+          -- eapply fAll_sat; eauto. intros phi (b & j & <- & HH) % in_mapi_iff.
+             rewrite <- plus_n_O. destruct b; cbn.
+             rewrite <- nth_default_eq. unfold nth_default. now rewrite HH.
+             rewrite <- nth_default_eq. unfold nth_default. destruct (nthe j l); congruence.
+        * now eapply omniscient_to_classical.
+    - pose (g := fun n : nat => f n Vector.nil).
+      exists g. intros n. unfold Th in H.
+      specialize (H (phi n) ltac:(unfold contains; eauto)).
+      assert ( forall l, forall phi0 : form, phi0 el mapi (fun (i : nat) (b : bool) => if b then @Pred count_sig i Vector.nil else Neg (@Pred count_sig i Vector.nil)) l 0 -> forall rho0 : env D, dec (rho0 ⊨ phi0)) as HHH by shelve.
+      eapply fExists_sat' in H as (phi' & H1 & H); eauto.
+      eapply in_map_iff in H1 as (l & <- & [H3 H4] % in_filter_iff).
+      rewrite fAll_sat' in H.
+      destruct (listable_list_length n) as [L HL].
+      cbn in *. eapply HL in H3.
+      enough (l = [g p | p ∈ seq 0 n]) as -> by now eapply HD.
+      subst. clear - H decI standI.
+      revert H. generalize 0 as n.
+      induction l; cbn; intros.
+      + reflexivity.
+      + f_equal. destruct a.
+        * pose proof (H (@Pred count_sig n Vector.nil) (or_introl eq_refl)) as H0.
+          eapply decI in H0. unfold g. cbn in H0. now rewrite H0.
+        * pose proof (H (Neg (@Pred count_sig n Vector.nil)) (or_introl eq_refl)) as H0.
+          cbn in H0. unfold g. rewrite <- decI in H0.
+          symmetry. eapply not_true_is_false.
+          intros [] % H0 % standI.
+        * eapply IHl. intros. eapply H. eauto.
+      + eauto.
+      + eauto. 
+      + intros phi0 ? % in_map_iff. clear - H2 standI decI HHH.
+        induction filter.
+        * exfalso. destruct H2 as (? & ? & ?); cbn in *; congruence.
+        * decide (phi0 = fAll (mapi (fun (i : nat) (b : bool) => if b then @Pred count_sig i Vector.nil else Neg (@Pred count_sig i Vector.nil)) a 0)).
+          -- subst. intros.
+             eapply omniscient_on_fAll_sat. eauto. eapply HHH. 
+          -- eapply IHl. destruct H2 as (? & ? & ?). destruct H0.
+             ++ subst. congruence.
+             ++ eauto.
+                Unshelve. {
+                  intros ? ? ? % in_mapi_iff. clear - H1 standI decI.
+                  revert H1.
+                  generalize 0 as k.
+                  induction l; intros k H1.
+                  * exfalso. destruct H1 as (? & [] & ? & ?); cbn in *; congruence.
+                  * decide (phi0 = @Pred count_sig k Vector.nil).
+                    -- subst. intros. destruct (f k Vector.nil) eqn:E.
+                       left. eapply decI. eauto. right. intros ? % decI. cbn in *. congruence.
+                    -- decide (phi0 = Neg (@Pred count_sig k Vector.nil)).
+                       ++ subst. intros. destruct (f k Vector.nil) eqn:E.
+                          right. eapply decI in E. cbn. firstorder. left.
+                          intros ? % decI. cbn in *. congruence.
+                       ++ eapply (IHl (S k)).
+                          destruct H1 as (x & j & ? & ?).
+                          destruct j.
+                          ** cbn in H0. destruct x.
+                             --- inv H0. cbn in n. congruence.
+                             --- inv H0. cbn in n0. congruence.
+                          ** cbn in *. exists x, j; destruct x; subst; split; eauto; repeat f_equal; lia.
+                }
+  Qed.
+
+End WKL.
+
+Theorem compact_implies_WKL :
+  compactness (@DM) -> forall T : tree, infinite_tree T -> infinite_path T.
+Proof.
+  intros.
+  pose proof (tree_dec T) as [f Hf].
+  eapply compact_DM_WKL with (T_D := f); eauto. 
+  firstorder.
+Qed.
+Print Assumptions compact_implies_WKL.
